Tealeaves/Classes/Multisorted/Theory/Foldmap.v
@@ -1,0 +1,234 @@
+ From Tealeaves Require Import
+   Classes.Multisorted.DecoratedTraversableMonad
+   Classes.Multisorted.Theory.Container
+   Classes.Multisorted.Theory.Targeted
+   Functors.List
+   Functors.Subset
+   Functors.Constant.
+
+Import TypeFamily.Notations.
+Import Monoid.Notations.
+Import List.ListNotations.
+Import Misc.Subset.Notations.
+Import Multisorted.Theory.Container.Notations.
+#[local] Open Scope list_scope.
+
+#[local] Generalizable Variables A B C F G W T U K M.
+
+(** * Foldmap *)
+(******************************************************************************)
+
+(** ** Operations *)
+(******************************************************************************)
+Section foldmap.
+
+  Context
+    (U : Type -> Type)
+    `{MultiDecoratedTraversablePreModule W T U}
+    `{! MultiDecoratedTraversableMonad W T}
+    `{M_mn_op: Monoid_op M}
+    `{M_mn_unit: Monoid_unit M}.
+
+  Definition foldMapmd_gen {A} (fake: Type) (f : K -> (W * A) -> M): U A -> M :=
+    mmapdt (B := fake) U (const M) f.
+
+  Definition foldMapmd {A} (f : K -> (W * A) -> M): U A -> M :=
+    foldMapmd_gen False f.
+
+  Definition foldMapm {A} (f : K -> A -> M) : U A -> M :=
+    foldMapmd (f ◻ allK (extract (W := (prod W)))).
+
+  Definition foldMapkd {A} (k: K) (f : W * A -> M): U A -> M :=
+    foldMapmd (tgt_def k f (const Ƶ)).
+
+  Definition foldMapk {A} (k: K) (f : A -> M): U A -> M :=
+    foldMapm (tgt_def k f (const Ƶ)).
+
+  Lemma foldMapmd_to_mmapdt {A} (f : K -> (W * A) -> M):
+    foldMapmd f = mmapdt (B := False) U (const M) f.
+  Proof.
+    reflexivity.
+  Qed.
+
+  Lemma foldMapm_to_foldMapmd {A} (f : K -> A -> M):
+    foldMapm f = foldMapmd (f ◻ allK (extract (W := (prod W)))).
+  Proof.
+    reflexivity.
+  Qed.
+
+  Lemma foldMapkd_to_kmapdt {A} (f : W * A -> M) {k: K}:
+    foldMapkd k f = kmapdt U k (G := const M) f.
+  Proof.
+    unfold kmapdt.
+    unfold foldMapkd.
+    rewrite foldMapmd_to_mmapdt.
+  Admitted.
+
+  Lemma foldMapk_to_kmapt {A} (f : A -> M) {k: K}:
+    foldMapk k f = ktraverse U k (G := const M) f.
+  Proof.
+    unfold foldMapk.
+    unfold ktraverse.
+    rewrite foldMapm_to_foldMapmd.
+    rewrite foldMapmd_to_mmapdt.
+  Admitted.
+
+  Lemma foldMapk_to_foldMapkd {A} (f : A -> M) {k: K}:
+    foldMapk k f = foldMapkd k (f ∘ extract (W := prod W)).
+  Proof.
+  Admitted.
+
+End foldmap.
+
+Section tolist_and_tosubset.
+
+  Context
+    (U : Type -> Type)
+    `{MultiDecoratedTraversablePreModule W T U}
+    `{! MultiDecoratedTraversableMonad W T}.
+
+  Lemma tolistmd_gen_to_foldMapmd_gen : forall {A} {fake:Type} (t: U A),
+      tolistmd_gen U fake t = foldMapmd_gen U fake tolistmd_gen_loc t.
+  Proof.
+    reflexivity.
+  Qed.
+
+  Lemma tolistmd_to_foldMapmd : forall {A},
+      tolistmd (A := A) (T := T) U = foldMapmd U tolistmd_gen_loc.
+  Proof.
+    reflexivity.
+  Qed.
+
+  Definition tosetmd_gen_loc {A}: K -> W * A -> subset (W * (K * A)) :=
+    fun k '(w, a) => {{ (w, (k, a)) }}.
+
+  Lemma tosetmd_to_foldMapmd : forall {A},
+      tosetmd (A := A) (T := T) U = foldMapmd U tosetmd_gen_loc.
+  Proof.
+    intros.
+    unfold tosetmd.
+    rewrite tolistmd_to_foldMapmd.
+    unfold foldMapmd, foldMapmd_gen, mmapdt.
+    change (ContainerFunctor.tosubset (A := (W * (K * A))))
+      with (const (ContainerFunctor.tosubset (A := (W * (K * A))))
+              (list (W * (K * A)))).
+    Set Keyed Unification.
+    rewrite (dtp_mbinddt_morphism W T U
+                 (const (list (W * (K * A))))
+                 (const (subset (W * (K * A))))
+                 (H6 := ApplicativeMorphism_monoid_morphism)).
+    Unset Keyed Unification.
+    fequal.
+    ext j (w, a).
+    ext (j', (w', a')).
+    unfold vec_compose, compose, mapMret, vec_apply, const.
+    unfold_ops @Map_const.
+    unfold tosetmd_gen_loc,
+      tolistmd_gen_loc.
+    propext; intuition.
+  Qed.
+
+  #[global] Instance ApplicativeMorphism_filterk : forall {A} (k: K),
+      ApplicativeMorphism (const (list (W * (K * A))))
+                          (const (list (W * A)))
+                          (const (filterk k)).
+  Proof.
+    intros. eapply ApplicativeMorphism_monoid_morphism.
+    Unshelve. constructor; try typeclasses eauto.
+    - easy.
+    - intros. apply filterk_app.
+  Qed.
+
+  Lemma toklistd_to_foldMapkd : forall {A} (k: K),
+      toklistd (T := T) (A := A) U k = foldMapkd U k (fun p => [p]).
+    Proof.
+      intros.
+      unfold toklistd.
+      rewrite tolistmd_to_foldMapmd.
+      unfold foldMapmd, foldMapmd_gen, mmapdt.
+      rewrite (dtp_mbinddt_morphism W T U
+                 (const (list (W * (K * A))))
+                 (const (list (W * A)))
+                 (H6 := ApplicativeMorphism_filterk k)).
+      unfold foldMapkd, foldMapmd, foldMapmd_gen, mmapdt.
+      fequal. ext j (w, a).
+      unfold vec_compose, compose, mapMret, vec_apply, tgt_def.
+      cbn. destruct_eq_args k j.
+    Qed.
+
+  Lemma toksetd_to_foldMapkd : forall {A} (t: U A) (k : K),
+      toksetd U k t = foldMapkd U k (fun p => {{p}}) t.
+  Proof.
+    intros.
+    unfold toksetd.
+    rewrite toklistd_to_foldMapkd.
+    unfold foldMapmd, foldMapmd_gen, mmapdt.
+    change (ContainerFunctor.tosubset (A := (W * A)))
+      with (const (ContainerFunctor.tosubset (A := (W * A)))
+              (list (W * A))).
+    Set Keyed Unification.
+    rewrite (dtp_mbinddt_morphism W T U
+               (const (list (W * A)))
+               (const (subset (W * A)))
+               (H6 := ApplicativeMorphism_monoid_morphism)).
+    Unset Keyed Unification.
+    unfold foldMapkd, foldMapmd, foldMapmd_gen, mmapdt.
+    fequal.
+    ext j (w, a).
+    ext (w', a').
+    unfold vec_compose, compose, mapMret, vec_apply, const.
+    unfold_ops @Map_const.
+    unfold tgt_def.
+    propext; destruct_eq_args k j; intuition.
+  Qed.
+
+End tolist_and_tosubset.
+
+Section forall_and_exists.
+
+  Context
+    (U : Type -> Type)
+    `{MultiDecoratedTraversablePreModule W T U}
+    `{! MultiDecoratedTraversableMonad W T}.
+
+  Definition Forallmd {A} (P: K -> W * A -> Prop) :=
+    foldMapmd U (T := T)
+      (M_mn_op := Monoid_op_and) (M_mn_unit := Monoid_unit_true) P.
+
+  Definition Forallkd {A} (k: K) (P: W * A -> Prop) :=
+    foldMapkd U k (T := T)
+      (M_mn_op := Monoid_op_and) (M_mn_unit := Monoid_unit_true) P.
+
+  Lemma Forallmd_to_foldMapmd {A} (P: K -> W * A -> Prop ):
+    Forallmd P =
+    foldMapmd U (T := T)
+      (M_mn_op := Monoid_op_and) (M_mn_unit := Monoid_unit_true) P.
+  Proof.
+    reflexivity.
+  Qed.
+
+  Lemma Forallkd_to_foldMapkd {A} (k: K) (P: W * A -> Prop):
+    Forallkd k P =
+    foldMapkd U k (T := T)
+      (M_mn_op := Monoid_op_and) (M_mn_unit := Monoid_unit_true) P.
+  Proof.
+    reflexivity.
+  Qed.
+
+  Definition Forallmd_spec : forall {A} (P: W * (K * A) -> Prop) (t: U A),
+      (forall w k a, (w, (k, a)) ∈md t -> P (w, (k, a))) <->
+        Forallmd (fun k '(w, a) => P (w, (k, a))) t.
+  Proof.
+    intros.
+    unfold Forallmd.
+  Admitted.
+
+  Definition Forallkd_spec : forall {A} {k: K} (P: W * A -> Prop) (t: U A),
+      (forall w a, (w, (k, a)) ∈md t -> P (w, a)) <->
+        Forallkd k (fun '(w, a) => P (w, a)) t.
+  Proof.
+    intros.
+    unfold Forallmd.
+  Admitted.
+
+End forall_and_exists.
