Tealeaves/Simplification/Tests/SystemF_Binddt.v
@@ -1,19 +1,20 @@
 From Tealeaves Require Export
   Examples.SystemF.Syntax
   Simplification.Tests.Support
-  Simplification.MBinddt.
+  Classes.Multisorted.Theory.Foldmap.
 
-Ltac cbn_mbinddt_post_hook ::=
-  try match goal with
-  | |- context[bind_type ?G ?f ?τ] =>
-      change (bind_type G f τ) with (mbinddt typ G f τ)
-  | |- context[bind_term ?G ?f ?t] =>
-      change (bind_term G f t) with (mbinddt term G f t)
-  end.
-
-#[local] Generalizable Variables G.
+#[local] Generalizable Variables G M.
 #[local] Arguments mbinddt {ix} {W}%type_scope {T} U%function_scope
   {MBind} {F}%function_scope {H H0 H1 A B} _ _.
+
+Ltac tactic_being_tested := idtac.
+
+Ltac test_simplification :=
+  intros;
+  tactic_being_tested;
+  try normalize_K;
+  conclude.
+
 
 (** ** <<mbinddt>> *)
 (******************************************************************************)
@@ -23,43 +24,38 @@ Section rw_mbinddt.
     (A B : Type)
     `{Applicative G}
     (f : forall k, list K * A -> G (SystemF k B)).
-
-  Ltac test_mbinddt :=
-    intros;
-    cbn_mbinddt;
-    try normalize_K;
-    conclude.
+  Ltac tactic_being_tested ::= cbn_mbinddt.
 
   Lemma mbinddt_type_rw1 : forall c,
       mbinddt typ f (ty_c c) = pure (ty_c c).
   Proof.
-    test_mbinddt.
+    test_simplification.
   Qed.
 
   Lemma mbinddt_type_rw2 : forall (a : A),
       mbinddt typ f (ty_v a) = f ktyp (nil, a).
   Proof.
-    test_mbinddt.
+    test_simplification.
   Qed.
 
   Lemma mbinddt_type_rw3 : forall (t1 t2 : typ A),
       mbinddt typ f (ty_ar t1 t2) =
         pure ty_ar <⋆> mbinddt typ f t1 <⋆> mbinddt typ f t2.
   Proof.
-    test_mbinddt.
+    test_simplification.
   Qed.
 
   Lemma mbinddt_type_rw4 : forall (body : typ A),
       mbinddt typ f (ty_univ body) =
         pure ty_univ <⋆> mbinddt typ (f ◻ allK (incr [ktyp])) body.
   Proof.
-    test_mbinddt.
+    test_simplification.
   Qed.
 
   Lemma mbinddt_term_rw1 : forall (a : A),
       mbinddt term f (tm_var a) = f ktrm (nil, a).
   Proof.
-    test_mbinddt.
+    test_simplification.
   Qed.
 
   Lemma mbinddt_term_rw2 : forall (τ : typ A) (t : term A),
@@ -67,28 +63,28 @@ Section rw_mbinddt.
         pure tm_abs <⋆> mbinddt typ f τ <⋆>
           mbinddt term (f ◻ allK (incr [ktrm])) t.
   Proof.
-    test_mbinddt.
+    test_simplification.
   Qed.
 
   Lemma mbinddt_term_rw3 : forall (t1 t2 : term A),
       mbinddt term f (tm_app t1 t2) =
         pure tm_app <⋆> (mbinddt term f t1) <⋆> (mbinddt term f t2).
   Proof.
-    test_mbinddt.
+    test_simplification.
   Qed.
 
   Lemma mbinddt_term_rw4 : forall (t : term A),
       mbinddt term f (tm_tab t) =
         pure tm_tab <⋆> mbinddt term (f ◻ allK (incr [ktyp])) t.
   Proof.
-    test_mbinddt.
+    test_simplification.
   Qed.
 
   Lemma mbinddt_term_rw5 : forall (t: term A) (τ : typ A),
       mbinddt term f (tm_tap t τ) =
         pure tm_tap <⋆> mbinddt term f t <⋆> mbinddt typ f τ.
   Proof.
-    test_mbinddt.
+    test_simplification.
   Qed.
 
 End rw_mbinddt.
@@ -101,42 +97,38 @@ Section rw_mbindd.
     (A B : Type)
     (f : forall k, list K * A -> SystemF k B).
 
-  Ltac test_mbindd :=
-    intros;
-    simplify_mbindd;
-    try normalize_K;
-    conclude.
+  Ltac tactic_being_tested ::= simplify_mbindd.
 
   Lemma mbindd_type_rw1 : forall c,
       mbindd typ f (ty_c c) = ty_c c.
   Proof.
-    test_mbindd.
+    test_simplification.
   Qed.
 
   Lemma mbindd_type_rw2 : forall (a : A),
       mbindd typ f (ty_v a) = f ktyp (nil, a).
   Proof.
-    test_mbindd.
+    test_simplification.
   Qed.
 
   Lemma mbindd_type_rw3 : forall (t1 t2 : typ A),
       mbindd typ f (ty_ar t1 t2) =
         ty_ar (mbindd typ f t1) (mbindd typ f t2).
   Proof.
-    test_mbindd.
+    test_simplification.
   Qed.
 
   Lemma mbindd_type_rw4 : forall (body : typ A),
       mbindd typ f (ty_univ body) =
         ty_univ (mbindd typ (f ◻ allK (incr [ktyp])) body).
   Proof.
-    test_mbindd.
+    test_simplification.
   Qed.
 
   Lemma mbindd_term_rw1 : forall (a : A),
       mbindd term f (tm_var a) = f ktrm (nil, a).
   Proof.
-    test_mbindd.
+    test_simplification.
   Qed.
 
   Lemma mbindd_term_rw2 : forall (τ : typ A) (t : term A),
@@ -144,361 +136,541 @@ Section rw_mbindd.
         tm_abs (mbindd typ f τ)
           (mbindd term (f ◻ allK (incr [ktrm])) t).
   Proof.
-    test_mbindd.
+    test_simplification.
   Qed.
 
   Lemma mbindd_term_rw3 : forall (t1 t2 : term A),
       mbindd term f (tm_app t1 t2) =
-        tm_app  (mbindd term f t1) (mbindd term f t2).
+        tm_app (mbindd term f t1) (mbindd term f t2).
   Proof.
-    test_mbindd.
+    test_simplification.
   Qed.
 
   Lemma mbindd_term_rw4 : forall (t : term A),
       mbindd term f (tm_tab t) =
         tm_tab (mbindd term (f ◻ allK (incr [ktyp])) t).
   Proof.
-    test_mbindd.
+    test_simplification.
   Qed.
 
   Lemma mbindd_term_rw5 : forall (t: term A) (τ : typ A),
       mbindd term f (tm_tap t τ) =
         tm_tap (mbindd term f t) (mbindd typ f τ).
   Proof.
-    test_mbindd.
+    test_simplification.
   Qed.
 
 End rw_mbindd.
 
-(** ** <<kbindd>> *)
+(** ** <<mbind>> *)
 (******************************************************************************)
-Section rw_kbindd.
-
-  Lemma kbindd_to_mbindd `{Ix:Index}: forall A (k: K) (f: list K * A -> SystemF k A),
-    kbindd typ k f = mbindd typ (btgd k f).
-  Proof.
-    reflexivity.
-  Qed.
-
-  Context
-    (A : Type)
-    (k : K2)
-    (f : list K2 * A -> SystemF k A).
-
-  Lemma btgd_compose_incr:
-    btgd k f ◻ allK (incr [ktyp]) =
-      btgd k (f ⦿ [ktyp]).
-  Proof.
-    intros.
-    ext j.
-    unfold allK, const.
-    unfold vec_compose.
-    compare values k and j.
-    { autorewrite with tea_tgt_eq.
-      reflexivity. }
-    { autorewrite with tea_tgt_neq.
-      reassociate -> on left.
-      rewrite extract_incr.
-      reflexivity. }
-  Qed.
-
-  Ltac simplify_kbindd :=
-    rewrite ?kbindd_to_mbindd;
-    simplify_mbindd;
-    rewrite <- ?kbindd_to_mbindd;
-    autorewrite* with tea_tgt;
-    try normalize_K.
-
-  Ltac test_kbindd :=
-    intros;
-    simplify_kbindd.
-
-  Lemma kbindd_type_rw1 : forall c,
-      kbindd typ k f (ty_c c) = ty_c c.
-  Proof.
-    test_kbindd.
-    conclude.
-  Qed.
-
-  Lemma kbindd_type_rw2 : forall (a : A),
-      kbindd typ k f (ty_v a) =
-        btgd k f ktyp ([], a).
-  Proof.
-    test_kbindd.
-    conclude.
-  Qed.
-
-  Lemma kbindd_type_rw3 : forall (t1 t2 : typ A),
-      kbindd typ k f (ty_ar t1 t2) =
-        ty_ar (kbindd typ k f t1) (kbindd typ k f t2).
-  Proof.
-    test_kbindd.
-    conclude.
-  Qed.
-
-  Lemma kbindd_type_rw4 : forall (body : typ A),
-      kbindd typ k f (ty_univ body) =
-        ty_univ (kbindd typ k (f ⦿ [ktyp]) body).
-  Proof.
-    intros.
-    simplify_kbindd.
-    setoid_rewrite btgd_compose_incr.
-    rewrite <- kbindd_to_mbindd.
-    normalize_K.
-    conclude.
-  Qed.
-
-  (*
-  Lemma kbindd_term_rw1 : forall (a : A),
-      kbindd term ktrm f (tm_var a) = f ktrm (nil, a).
-  Proof.
-    test_kbindd.
-  Qed.
-
-  Lemma kbindd_term_rw2 : forall (τ : typ A) (t : term A),
-      kbindd term k f (tm_abs τ t) =
-        tm_abs (kbindd typ k f τ)
-          (kbindd term k (f ◻ allK (incr [ktrm])) t).
-  Proof.
-    test_kbindd.
-  Qed.
-
-  Lemma kbindd_term_rw3 : forall (t1 t2 : term A),
-      kbindd term f (tm_app t1 t2) =
-        tm_app  (kbindd term f t1)  (kbindd term f t2).
-  Proof.
-    test_kbindd.
-  Qed.
-
-  Lemma kbindd_term_rw4 : forall (t : term A),
-      kbindd term f (tm_tab t) =
-        tm_tab (kbindd term (f ◻ allK (incr [ktyp])) t).
-  Proof.
-    test_kbindd.
-  Qed.
-
-  Lemma kbindd_term_rw5 : forall (t: term A) (τ : typ A),
-      kbindd term f (tm_tap t τ) =
-        tm_tap (kbindd term f t) (kbindd typ f τ).
-  Proof.
-    test_kbindd.
-  Qed.
-  *)
-
-End rw_kbindd.
-
-(*
-(** * Rewriting operations on <<typ>> *)
-(******************************************************************************)
-
-(** ** Fundamental operations *)
-(******************************************************************************)
-
-(** *** <<mmapdt>> *)
-(******************************************************************************)
-Section rw_mmapdt_type.
+Section rw_mbind.
 
   Context
     (A B : Type)
-    `{Applicative F}
-    (f : K -> list K * A -> F B).
+    (f : forall k, A -> SystemF k B).
 
-  Lemma rw_mmapdt_type1:
-    forall c, mmapdt typ F f (ty_c c) = pure (ty_c c).
+  Ltac tactic_being_tested ::= simplify_mbind.
+
+  Lemma mbind_type_rw1 : forall c,
+      mbind typ f (ty_c c) = ty_c c.
+  Proof.
+    test_simplification.
+  Qed.
+
+  Lemma mbind_type_rw2 : forall (a : A),
+      mbind typ f (ty_v a) = f ktyp a.
+  Proof.
+    test_simplification.
+  Qed.
+
+  Lemma mbind_type_rw3 : forall (t1 t2 : typ A),
+      mbind typ f (ty_ar t1 t2) =
+        ty_ar (mbind typ f t1) (mbind typ f t2).
+  Proof.
+    test_simplification.
+  Qed.
+
+  Lemma mbind_type_rw4 : forall (body : typ A),
+      mbind typ f (ty_univ body) =
+        ty_univ (mbind typ f body).
+  Proof.
+    test_simplification.
+  Qed.
+
+  Lemma mbind_term_rw1 : forall (a : A),
+      mbind term f (tm_var a) = f ktrm a.
+  Proof.
+    test_simplification.
+  Qed.
+
+  Lemma mbind_term_rw2 : forall (τ : typ A) (t : term A),
+      mbind term f (tm_abs τ t) =
+        tm_abs (mbind typ f τ) (mbind term f t).
+  Proof.
+    test_simplification.
+  Qed.
+
+  Lemma mbind_term_rw3 : forall (t1 t2 : term A),
+      mbind term f (tm_app t1 t2) =
+        tm_app (mbind term f t1) (mbind term f t2).
+  Proof.
+    test_simplification.
+  Qed.
+
+  Lemma mbind_term_rw4 : forall (t : term A),
+      mbind term f (tm_tab t) =
+        tm_tab (mbind term f t).
+  Proof.
+    test_simplification.
+  Qed.
+
+  Lemma mbind_term_rw5 : forall (t: term A) (τ : typ A),
+      mbind term f (tm_tap t τ) =
+        tm_tap (mbind term f t) (mbind typ f τ).
+  Proof.
+    test_simplification.
+  Qed.
+
+End rw_mbind.
+
+(** ** <<mmapdt>> *)
+(******************************************************************************)
+Section rw_mmapdt.
+
+  Context
+    (A B : Type)
+    `{Applicative G}
+    (f : forall (k: K), list K * A -> G B).
+
+  Ltac tactic_being_tested ::= simplify_mmapdt.
+
+  Lemma mmapdt_type_rw1 : forall c,
+      mmapdt typ G f (ty_c c) = pure (ty_c c).
+  Proof.
+    test_simplification.
+  Qed.
+
+  Lemma mmapdt_type_rw2 : forall (a : A),
+      mmapdt typ G f (ty_v a) = pure ty_v <⋆> f ktyp (nil, a).
   Proof.
     intros.
-    rewrite mmapdt_to_mbinddt.
-    simplify.
+    simplify_mmapdt.
     reflexivity.
   Qed.
 
-  (* Why is this expressed with ? *)
-  Lemma rw_mmapdt_type2: forall (a: A), mmapdt typ F f (ty_v a) = pure ty_v  f ktyp (nil, a).
+  Lemma mmapdt_type_rw3 : forall (t1 t2 : typ A),
+      mmapdt typ G f (ty_ar t1 t2) =
+        pure ty_ar <⋆> mmapdt typ G f t1 <⋆> mmapdt typ G f t2.
+  Proof.
+    test_simplification.
+  Qed.
+
+  Lemma mmapdt_type_rw4 : forall (body : typ A),
+      mmapdt typ G f (ty_univ body) =
+        pure ty_univ <⋆> mmapdt typ G (f ◻ allK (incr [ktyp])) body.
+  Proof.
+    test_simplification.
+  Qed.
+
+  Lemma mmapdt_term_rw1 : forall (a : A),
+      mmapdt term G f (tm_var a) = pure tm_var <⋆> f ktrm (nil, a).
   Proof.
     intros.
-    rewrite mmapdt_to_mbinddt.
-    simplify.
-    rewrite <- map_to_ap.
+    simplify_mmapdt.
     reflexivity.
   Qed.
 
-  Lemma rw_mmapdt_type3: forall (t1 t2: typ A),
-      mmapdt typ F f (ty_ar t1 t2) =
-        pure (ty_ar)  mmapdt typ F f t1  mmapdt typ F f t2.
+  Lemma mmapdt_term_rw2 : forall (τ : typ A) (t : term A),
+      mmapdt term G f (tm_abs τ t) =
+        pure tm_abs <⋆> mmapdt typ G f τ <⋆>
+          mmapdt term G (f ◻ allK (incr [ktrm])) t.
   Proof.
-    intros.
-    rewrite mmapdt_to_mbinddt.
-    simplify.
-    reflexivity.
+    test_simplification.
   Qed.
 
-  Lemma rw_mmapdt_type4: forall (body: typ A),
-      mmapdt typ F f (ty_univ body) =
-        pure (ty_univ)  mmapdt typ F (fun k => f k ∘ incr [ktyp]) body.
+  Lemma mmapdt_term_rw3 : forall (t1 t2 : term A),
+      mmapdt term G f (tm_app t1 t2) =
+        pure tm_app <⋆> mmapdt term G f t1 <⋆> mmapdt term G f t2.
   Proof.
-    reflexivity.
+    test_simplification.
   Qed.
 
-End rw_mmapdt_type.
+  Lemma mmapdt_term_rw4 : forall (t : term A),
+      mmapdt term G f (tm_tab t) =
+        pure tm_tab <⋆> mmapdt term G (f ◻ allK (incr [ktyp])) t.
+  Proof.
+    test_simplification.
+  Qed.
 
-(*
-#[export] Hint Rewrite @rw_mmapdt_type1 @rw_mmapdt_type2 @rw_mmapdt_type3 @rw_mmapdt_type4: sysf_rw.
-*)
+  Lemma mmapdt_term_rw5 : forall (t: term A) (τ : typ A),
+      mmapdt term G f (tm_tap t τ) =
+        pure tm_tap <⋆> mmapdt term G f t <⋆> mmapdt typ G f τ.
+  Proof.
+    test_simplification.
+  Qed.
 
-(** *** <<mbindd>> *)
+End rw_mmapdt.
+
+(** ** <<mmapd>> *)
 (******************************************************************************)
-Section rw_mbindd_type.
+Section rw_mmapd.
 
   Context
-    (A B: Type)
-    (f: forall k, list K * A -> SystemF k B).
+    (A B : Type)
+    (f : forall (k: K), list K * A -> B).
 
-  Lemma rw_mbindd_type1: forall c, mbindd typ f (ty_c c) = ty_c c.
-  Proof. reflexivity. Qed.
+  Ltac tactic_being_tested ::= simplify_mmapd.
 
-  Lemma rw_mbindd_type2: forall (a: A), mbindd typ f (ty_v a) = f ktyp (nil, a).
-  Proof. reflexivity. Qed.
-
-  Lemma rw_mbindd_type3: forall (t1 t2: typ A), mbindd typ f (ty_ar t1 t2) = ty_ar (mbindd typ f t1) (mbindd typ f t2).
-  Proof. reflexivity. Qed.
-
-  Lemma rw_mbindd_type4: forall (body: typ A), mbindd typ f (ty_univ body) = ty_univ (mbindd typ (fun k => f k ∘ incr [ktyp]) body).
-  Proof. reflexivity. Qed.
-
-End rw_mbindd_type.
-
-#[export] Hint Rewrite @rw_mbindd_type1 @rw_mbindd_type2 @rw_mbindd_type3 @rw_mbindd_type4: sysf_rw.
-
-(** *** <<mbind>> *)
-(******************************************************************************)
-Section rw_mbind_type.
-
-  Context
-    (A B: Type)
-    (f: forall k, A -> SystemF k B).
-
-  Lemma rw_mbind_type1: forall c, mbind typ f (ty_c c) = ty_c c.
-  Proof. reflexivity. Qed.
-
-  Lemma rw_mbind_type2: forall (a: A), mbind typ f (ty_v a) = f ktyp a.
-  Proof. reflexivity. Qed.
-
-  Lemma rw_mbind_type3: forall (t1 t2: typ A), mbind typ f (ty_ar t1 t2) = ty_ar (mbind typ f t1) (mbind typ f t2).
-  Proof. reflexivity. Qed.
-
-  Lemma rw_mbind_type4: forall (body: typ A), mbind typ f (ty_univ body) = ty_univ (mbind typ f body).
+  Lemma mmapd_type_rw1 : forall c,
+      mmapd typ f (ty_c c) = pure (ty_c c).
   Proof.
-    intros. unfold mbind. rewrite rw_mbindd_type4. repeat fequal. now ext k [w a].
+    test_simplification.
   Qed.
 
-End rw_mbind_type.
-
-#[export] Hint Rewrite @rw_mbind_type1 @rw_mbind_type2 @rw_mbind_type3 @rw_mbind_type4: sysf_rw.
-
-(** *** <<kbindd>> with <<ktyp>> *)
-(******************************************************************************)
-Section rw_kbindd_type.
-
-  Context
-    (A: Type)
-    (f: list K * A -> typ A).
-
-  Lemma rw_kbindd_ktyp_type1: forall c, kbindd typ ktyp f (ty_c c) = ty_c c.
-  Proof. reflexivity. Qed.
-
-  Lemma rw_kbindd_ktyp_type2: forall a, kbindd typ ktyp f (ty_v a) = f (nil, a).
-  Proof. reflexivity. Qed.
-
-  Lemma rw_kbindd_ktyp_type3: forall (t1 t2: typ A), kbindd typ ktyp f (ty_ar t1 t2) = ty_ar (kbindd typ ktyp f t1) (kbindd typ ktyp f t2).
-  Proof. reflexivity. Qed.
-
-  Lemma rw_kbindd_ktyp_type4: forall (body: typ A), kbindd typ ktyp f (ty_univ body) = ty_univ (kbindd typ ktyp (f ∘ incr [ktyp]) body).
+  Lemma mmapd_type_rw2 : forall (a : A),
+      mmapd typ f (ty_v a) = ty_v (f ktyp (nil, a)).
   Proof.
-    intros. unfold kbindd. simpl_F.
-    do 2 fequal. now ext j [w a].
+    test_simplification.
   Qed.
 
-End rw_kbindd_type.
-
-#[export] Hint Rewrite @rw_kbindd_ktyp_type1 @rw_kbindd_ktyp_type2 @rw_kbindd_ktyp_type3 @rw_kbindd_ktyp_type4: sysf_rw.
-
-(** *** <<kbindd>> with <<ktrm>> *)
-(******************************************************************************)
-Section rw_kbindd_type.
-
-  Context
-    (A: Type)
-    (f: list K * A -> term A).
-
-  Lemma rw_kbindd_ktrm_type1: forall c, kbindd typ ktrm f (ty_c c) = ty_c c.
-  Proof. reflexivity. Qed.
-
-  Lemma rw_kbindd_ktrm_type2: forall a, kbindd typ ktrm f (ty_v a) = ty_v a.
-  Proof. reflexivity. Qed.
-
-  Lemma rw_kbindd_ktrm_type3: forall (t1 t2: typ A), kbindd typ ktrm f (ty_ar t1 t2) = ty_ar (kbindd typ ktrm f t1) (kbindd typ ktrm f t2).
-  Proof. reflexivity. Qed.
-
-  Lemma rw_kbindd_ktrm_type4: forall (body: typ A), kbindd typ ktrm f (ty_univ body) = ty_univ (kbindd typ ktrm (f ∘ incr [ktyp]) body).
+  Lemma mmapd_type_rw3 : forall (t1 t2 : typ A),
+      mmapd typ f (ty_ar t1 t2) =
+        ty_ar (mmapd typ f t1) (mmapd typ f t2).
   Proof.
-    intros. unfold kbindd. simpl_F.
-    do 2 fequal. now ext j [w a].
+    test_simplification.
   Qed.
 
-End rw_kbindd_type.
-
-#[export] Hint Rewrite @rw_kbindd_ktrm_type1 @rw_kbindd_ktrm_type2 @rw_kbindd_ktrm_type3 @rw_kbindd_ktrm_type4: sysf_rw.
-
-(** *** <<kbind>> with <<ktyp>> *)
-(******************************************************************************)
-Section rw_kbind_type.
-
-  Context
-    (A: Type)
-    (f: A -> typ A).
-
-  Lemma rw_kbind_ktyp_type1: forall c, kbind typ ktyp f (ty_c c) = ty_c c.
-  Proof. reflexivity. Qed.
-
-  Lemma rw_kbind_ktyp_type2: forall a, kbind typ ktyp f (ty_v a) = f a.
-  Proof. reflexivity. Qed.
-
-  Lemma rw_kbind_ktyp_type3: forall (t1 t2: typ A), kbind typ ktyp f (ty_ar t1 t2) = ty_ar (kbind typ ktyp f t1) (kbind typ ktyp f t2).
-  Proof. reflexivity. Qed.
-
-  Lemma rw_kbind_ktyp_type4: forall (body: typ A), kbind typ ktyp f (ty_univ body) = ty_univ (kbind typ ktyp f body).
+  Lemma mmapd_type_rw4 : forall (body : typ A),
+      mmapd typ f (ty_univ body) =
+        ty_univ (mmapd typ (f ◻ allK (incr [ktyp])) body).
   Proof.
-    intros. unfold kbind. now simpl_F.
+    test_simplification.
   Qed.
 
-End rw_kbind_type.
-
-#[export] Hint Rewrite @rw_kbind_ktyp_type1 @rw_kbind_ktyp_type2 @rw_kbind_ktyp_type3 @rw_kbind_ktyp_type4: sysf_rw.
-
-(** *** <<kbind>> with <<ktrm>> *)
-(******************************************************************************)
-Section rw_kbind_type.
-
-  Context
-    (A: Type)
-    (f: A -> term A).
-
-  Lemma rw_kbind_ktrm_type1: forall c, kbind typ ktrm f (ty_c c) = ty_c c.
-  Proof. reflexivity. Qed.
-
-  Lemma rw_kbind_ktrm_type2: forall a, kbind typ ktrm f (ty_v a) = ty_v a.
-  Proof. reflexivity. Qed.
-
-  Lemma rw_kbind_ktrm_type3: forall (t1 t2: typ A), kbind typ ktrm f (ty_ar t1 t2) = ty_ar (kbind typ ktrm f t1) (kbind typ ktrm f t2).
-  Proof. reflexivity. Qed.
-
-  Lemma rw_kbind_ktrm_type4: forall (body: typ A), kbind typ ktrm f (ty_univ body) = ty_univ (kbind typ ktrm f body).
+  Lemma mmapd_term_rw1 : forall (a : A),
+      mmapd term f (tm_var a) = tm_var (f ktrm (nil, a)).
   Proof.
-    intros. unfold kbind. now simpl_F.
+    test_simplification.
   Qed.
 
-End rw_kbind_type.
+  Lemma mmapd_term_rw2 : forall (τ : typ A) (t : term A),
+      mmapd term f (tm_abs τ t) =
+        tm_abs (mmapd typ f τ)
+          (mmapd term (f ◻ allK (incr [ktrm])) t).
+  Proof.
+    test_simplification.
+  Qed.
 
-#[export] Hint Rewrite @rw_kbind_ktrm_type1 @rw_kbind_ktrm_type2 @rw_kbind_ktrm_type3 @rw_kbind_ktrm_type4: sysf_rw.
+  Lemma mmapd_term_rw3 : forall (t1 t2 : term A),
+      mmapd term f (tm_app t1 t2) =
+        tm_app (mmapd term f t1) (mmapd term f t2).
+  Proof.
+    test_simplification.
+  Qed.
 
-*)
+  Lemma mmapd_term_rw4 : forall (t : term A),
+      mmapd term f (tm_tab t) =
+        tm_tab (mmapd term (f ◻ allK (incr [ktyp])) t).
+  Proof.
+    test_simplification.
+  Qed.
+
+  Lemma mmapd_term_rw5 : forall (t: term A) (τ : typ A),
+      mmapd term f (tm_tap t τ) =
+        tm_tap (mmapd term f t) (mmapd typ f τ).
+  Proof.
+    test_simplification.
+  Qed.
+
+End rw_mmapd.
+
+Ltac simplify_foldMapmd_pre_refold_hook ix := idtac.
+Ltac simplify_foldMapmd_post_refold_hook M :=
+  repeat simplify_applicative_const;
+  (* ^ above step creates some ((Ƶ ● m) ● n) *)
+  repeat simplify_monoid_units;
+  change (@const Type Type M ?anything) with M.
+
+Ltac simplify_foldMapmd :=
+  match goal with
+  | |- context[foldMapmd (W := ?W) (T := ?T) (ix := ?ix) (M := ?M)
+                ?U ?f ?t] =>
+      rewrite ?foldMapmd_to_mmapdt;
+      simplify_mmapdt;
+      simplify_foldMapmd_pre_refold_hook ix;
+      rewrite <- ?foldMapmd_to_mmapdt;
+      simplify_foldMapmd_post_refold_hook M
+  end.
+
+(** ** <<foldMapmd>> *)
+(******************************************************************************)
+Section rw_foldMapmd.
+
+  Context
+    (A : Type)
+      `{Monoid M}
+      (f : forall (k: K), list K * A -> M).
+
+  Ltac tactic_being_tested ::= simplify_foldMapmd.
+
+  Lemma foldMapmd_type_rw1 : forall c,
+      foldMapmd typ f (ty_c c) = Ƶ.
+  Proof.
+    test_simplification.
+  Qed.
+
+  Lemma foldMapmd_type_rw2 : forall (a : A),
+      foldMapmd typ f (ty_v a) = f ktyp (nil, a).
+  Proof.
+    test_simplification.
+  Qed.
+
+  Lemma foldMapmd_type_rw3 : forall (t1 t2 : typ A),
+      foldMapmd typ f (ty_ar t1 t2) =
+        foldMapmd typ f t1 ● foldMapmd typ f t2.
+  Proof.
+    test_simplification.
+  Qed.
+
+  Lemma foldMapmd_type_rw4 : forall (body : typ A),
+      foldMapmd typ f (ty_univ body) =
+        foldMapmd typ (f ◻ allK (incr [ktyp])) body.
+  Proof.
+    test_simplification.
+  Qed.
+
+  Lemma foldMapmd_term_rw1 : forall (a : A),
+      foldMapmd term f (tm_var a) = f ktrm (nil, a).
+  Proof.
+    test_simplification.
+  Qed.
+
+  Lemma foldMapmd_term_rw2 : forall (τ : typ A) (t : term A),
+      foldMapmd term f (tm_abs τ t) =
+        foldMapmd typ f τ ●
+          foldMapmd term (f ◻ allK (incr [ktrm])) t.
+  Proof.
+    test_simplification.
+  Qed.
+
+  Lemma foldMapmd_term_rw3 : forall (t1 t2 : term A),
+      foldMapmd term f (tm_app t1 t2) =
+        foldMapmd term f t1 ● foldMapmd term f t2.
+  Proof.
+    test_simplification.
+  Qed.
+
+  Lemma foldMapmd_term_rw4 : forall (t : term A),
+      foldMapmd term f (tm_tab t) =
+        foldMapmd term (f ◻ allK (incr [ktyp])) t.
+  Proof.
+    test_simplification.
+  Qed.
+
+  Lemma foldMapmd_term_rw5 : forall (t: term A) (τ : typ A),
+      foldMapmd term f (tm_tap t τ) =
+        foldMapmd term f t ● foldMapmd typ f τ.
+  Proof.
+    test_simplification.
+  Qed.
+
+End rw_foldMapmd.
+
+(* after unfolding,
+   foldMapmd U (f ◻ allK extract) (C x1 x2)
+   is simplified to
+   foldMapmd typ ((f ◻ allK extract) ◻ allK (incr [ktyp])) x1) ...
+ *)
+Ltac simplify_foldMapm_pre_refold_hook ix :=
+  repeat ( rewrite ?vec_compose_assoc;
+           rewrite (vec_compose_allK (H := ix));
+           rewrite extract_incr).
+
+
+Ltac simplify_foldMapm_post_refold_hook ix := idtac.
+
+
+(* At a k-annotated leaf,
+   foldMapm f (Ret x)
+   becomes
+   (f ◻ allK (extract (W := ?W))) k (Ƶ, x)] =>
+ *)
+Ltac simplify_foldMapm_at_leaf_hook :=
+  simplify_mbind_at_leaf_hook.
+
+Ltac simplify_foldMapm :=
+  match goal with
+  | |- context[foldMapm (W := ?W) (T := ?T) (ix := ?ix) (M := ?M)
+                ?U ?f ?t] =>
+      rewrite ?foldMapm_to_foldMapmd;
+      simplify_foldMapmd;
+      simplify_foldMapm_pre_refold_hook ix;
+      rewrite <- ?foldMapm_to_foldMapmd;
+      simplify_foldMapm_post_refold_hook M;
+      simplify_foldMapm_at_leaf_hook
+  end.
+
+(** ** <<foldMapm>> *)
+(******************************************************************************)
+Section rw_foldMapm.
+
+  Context
+    (A : Type)
+      `{Monoid M}
+      (f : K -> A -> M).
+
+  Ltac tactic_being_tested ::= simplify_foldMapm.
+
+  Lemma foldMapm_type_rw1 : forall c,
+      foldMapm typ f (ty_c c) = Ƶ.
+  Proof.
+    test_simplification.
+  Qed.
+
+  Lemma foldMapm_type_rw2 : forall (a : A),
+      foldMapm typ f (ty_v a) = f ktyp a.
+  Proof.
+    test_simplification.
+  Qed.
+
+  Lemma foldMapm_type_rw3 : forall (t1 t2 : typ A),
+      foldMapm typ f (ty_ar t1 t2) =
+        foldMapm typ f t1 ● foldMapm typ f t2.
+  Proof.
+    test_simplification.
+  Qed.
+
+  Lemma foldMapm_type_rw4 : forall (body : typ A),
+      foldMapm typ f (ty_univ body) =
+        foldMapm typ f body.
+  Proof.
+    test_simplification.
+  Qed.
+
+  Lemma foldMapm_term_rw1 : forall (a : A),
+      foldMapm term f (tm_var a) = f ktrm a.
+  Proof.
+    test_simplification.
+  Qed.
+
+  Lemma foldMapm_term_rw2 : forall (τ : typ A) (t : term A),
+      foldMapm term f (tm_abs τ t) =
+        foldMapm typ f τ ●
+          foldMapm term f t.
+  Proof.
+    test_simplification.
+  Qed.
+
+  Lemma foldMapm_term_rw3 : forall (t1 t2 : term A),
+      foldMapm term f (tm_app t1 t2) =
+        foldMapm term f t1 ● foldMapm term f t2.
+  Proof.
+    test_simplification.
+  Qed.
+
+  Lemma foldMapm_term_rw4 : forall (t : term A),
+      foldMapm term f (tm_tab t) =
+        foldMapm term f t.
+  Proof.
+    test_simplification.
+  Qed.
+
+  Lemma foldMapm_term_rw5 : forall (t: term A) (τ : typ A),
+      foldMapm term f (tm_tap t τ) =
+        foldMapm term f t ● foldMapm typ f τ.
+  Proof.
+    test_simplification.
+  Qed.
+
+End rw_foldMapm.
+
+Ltac simplify_Forallmd_pre_refold_hook := idtac.
+Ltac simplify_Forallmd_post_refold_hook :=
+  unfold_ops @Monoid_op_and;
+  unfold_ops @Monoid_unit_true.
+
+Ltac simplify_Forallmd :=
+  match goal with
+  | |- context[Forallmd (W := ?W) (T := ?T) (ix := ?ix)
+                ?U ?f ?t] =>
+      rewrite ?Forallmd_to_foldMapmd;
+      simplify_foldMapmd;
+      simplify_Forallmd_pre_refold_hook;
+      rewrite <- ?Forallmd_to_foldMapmd;
+      simplify_Forallmd_post_refold_hook
+  end.
+
+(** ** <<Forallmd>> *)
+(******************************************************************************)
+Section rw_Forallmd.
+
+  Context
+    (A : Type)
+      `{Monoid M}
+      (f : forall (k: K), list K * A -> Prop).
+
+  Ltac tactic_being_tested ::= simplify_Forallmd.
+
+  Lemma Forallmd_type_rw1 : forall c,
+      Forallmd typ f (ty_c c) = True.
+  Proof.
+    test_simplification.
+  Qed.
+
+  Lemma Forallmd_type_rw2 : forall (a : A),
+      Forallmd typ f (ty_v a) = f ktyp (nil, a).
+  Proof.
+    test_simplification.
+  Qed.
+
+  Lemma Forallmd_type_rw3 : forall (t1 t2 : typ A),
+      Forallmd typ f (ty_ar t1 t2) =
+        (Forallmd typ f t1 /\ Forallmd typ f t2).
+  Proof.
+    test_simplification.
+  Qed.
+
+  Lemma Forallmd_type_rw4 : forall (body : typ A),
+      Forallmd typ f (ty_univ body) =
+        Forallmd typ (f ◻ allK (incr [ktyp])) body.
+  Proof.
+    test_simplification.
+  Qed.
+
+  Lemma Forallmd_term_rw1 : forall (a : A),
+      Forallmd term f (tm_var a) = f ktrm (nil, a).
+  Proof.
+    test_simplification.
+  Qed.
+
+  Lemma Forallmd_term_rw2 : forall (τ : typ A) (t : term A),
+      Forallmd term f (tm_abs τ t) =
+        (Forallmd typ f τ /\
+          Forallmd term (f ◻ allK (incr [ktrm])) t).
+  Proof.
+    test_simplification.
+  Qed.
+
+  Lemma Forallmd_term_rw3 : forall (t1 t2 : term A),
+      Forallmd term f (tm_app t1 t2) =
+        (Forallmd term f t1 /\ Forallmd term f t2).
+  Proof.
+    test_simplification.
+  Qed.
+
+  Lemma Forallmd_term_rw4 : forall (t : term A),
+      Forallmd term f (tm_tab t) =
+        Forallmd term (f ◻ allK (incr [ktyp])) t.
+  Proof.
+    test_simplification.
+  Qed.
+
+  Lemma Forallmd_term_rw5 : forall (t: term A) (τ : typ A),
+      Forallmd term f (tm_tap t τ) =
+        (Forallmd term f t /\ Forallmd typ f τ).
+  Proof.
+    test_simplification.
+  Qed.
+
+End rw_Forallmd.
