Tealeaves/Simplification/Tests/SystemF_LN.v
@@ -1,0 +1,911 @@
+From Tealeaves Require Export
+  Examples.SystemF.Syntax
+  Simplification.Tests.Support
+  Simplification.MBinddt
+  Simplification.Tests.SystemF_Binddt
+  Simplification.Tests.SystemF_Targeted
+  Classes.Multisorted.Theory.Foldmap.
+
+#[local] Generalizable Variables G.
+#[local] Arguments mbinddt {ix} {W}%type_scope {T} U%function_scope
+  {MBind} {F}%function_scope {H H0 H1 A B} _ _.
+
+#[local] Generalizable Variables A B C F W T U K.
+
+Section local_lemmas_needed.
+
+  Context
+    (U : Type -> Type)
+      `{MultiDecoratedTraversablePreModule (list K) T U
+          (mn_op := Monoid_op_list)
+          (mn_unit := Monoid_unit_list)}
+      `{! MultiDecoratedTraversableMonad (list K) T
+          (mn_op := Monoid_op_list)
+          (mn_unit := Monoid_unit_list)}.
+
+  Lemma subst_to_kbind : forall (k: K) (x: atom) (u: T k LN),
+      subst U k x u = kbind U k (subst_loc k x u).
+  Proof.
+    reflexivity.
+  Qed.
+
+  Lemma open_to_kbindd : forall (k: K) (u: T k LN),
+      open U k u = kbindd U k (open_loc k u).
+  Proof.
+    reflexivity.
+  Qed.
+
+  Lemma free_to_foldMapk : forall (k: K),
+      free U (T := T) k = foldMapk U k free_loc.
+  Proof.
+    intros.
+  Admitted.
+
+  Lemma FV_to_free : forall (k: K) (t: U LN),
+      FV U k t = atoms (free U (T := T) k t).
+  Proof.
+    reflexivity.
+  Qed.
+
+  Lemma LCn_to_Forallkd:
+    forall (n: nat) (t: U LN) k,
+      LCn U k n t = Forallkd U k (lc_loc k n) t.
+  Proof.
+    intros.
+    apply propositional_extensionality.
+    rewrite <- (Forallkd_spec U (lc_loc k n)).
+    reflexivity.
+  Qed.
+
+  Lemma LC_to_Forallkd:
+    forall (n: nat) (t: U LN) k,
+      LC U k t = Forallkd U k (lc_loc k 0) t.
+  Proof.
+    intros.
+    apply propositional_extensionality.
+    rewrite <- (Forallkd_spec U (lc_loc k 0)).
+    reflexivity.
+  Qed.
+
+  Lemma lc_loc_preincr_eq :
+    forall k n j,
+      k = j ->
+      (lc_loc k n ⦿ [j]) =
+        lc_loc k (S n).
+  Proof.
+    intros.
+    unfold preincr, compose, incr.
+    ext [w l].
+    unfold lc_loc.
+    destruct l as [x | m].
+    - reflexivity.
+    - cbn. destruct_eq_args k j.
+      propext; lia.
+  Qed.
+
+  Lemma lc_loc_preincr_neq :
+    forall k n j,
+      k <> j ->
+      (lc_loc k n ⦿ [j]) =
+        lc_loc k n.
+  Proof.
+    intros.
+    unfold preincr, compose, incr.
+    ext [w l].
+    unfold lc_loc.
+    destruct l as [x | m].
+    - reflexivity.
+    - cbn. destruct_eq_args k j.
+  Qed.
+
+End local_lemmas_needed.
+
+Create HintDb lc_loc_db.
+#[global] Hint Rewrite lc_loc_preincr_eq: lc_loc_db.
+#[global] Hint Rewrite lc_loc_preincr_neq: lc_loc_db.
+
+(*
+Ltac handle_lc_loc :=
+  autorewrite* with lc_loc_db using (auto; try discriminate).
+ *)
+
+Ltac handle_lc_loc :=
+  match goal with
+  | |- context[lc_loc (ix := ?ix)] =>
+      first [ rewrite (lc_loc_preincr_eq (ix := ix)) by auto
+            | rewrite (lc_loc_preincr_neq (ix := ix)) by
+              (solve [auto || discriminate])
+        ]
+  end.
+
+Ltac simplify_open_pre_refold_hook :=
+  idtac.
+
+Ltac simplify_open_post_refold_hook :=
+  idtac.
+
+Ltac simplify_open :=
+  rewrite ?open_to_kbindd;
+  simplify_kbindd;
+  simplify_open_pre_refold_hook;
+  rewrite <- ?open_to_kbindd;
+  simplify_open_post_refold_hook.
+
+(** ** <<open>> *)
+(******************************************************************************)
+Section rw_open.
+
+  Context
+    (A : Type)
+      (k : K2)
+      (x: atom)
+      (u: SystemF k LN).
+
+  Ltac tactic_being_tested ::= simplify_open.
+
+  Lemma open_type_rw1 : forall c,
+      open typ k u (ty_c c) = ty_c c.
+  Proof.
+    test_simplification.
+  Qed.
+
+  (*
+  Lemma open_type_rw2_neq : forall (a : A),
+      k <> ktyp ->
+      open typ k f (ty_v a) = ty_v a.
+  Proof.
+    intros.
+    simplify_open.
+    rewrite btgd_neq; auto.
+  Qed.*)
+
+  Lemma open_type_rw3 : forall (t1 t2 : typ LN),
+      open typ k u (ty_ar t1 t2) =
+        ty_ar (open typ k u t1) (open typ k u t2).
+  Proof.
+    test_simplification.
+  Qed.
+
+  Lemma open_type_rw4 : forall (body : typ LN),
+      open typ k u (ty_univ body) =
+        ty_univ (kbindd typ k (open_loc k u ⦿ [ktyp]) body).
+  Proof.
+    test_simplification.
+  Qed.
+
+  Lemma open_term_rw1_neq : forall (a : LN),
+      k <> ktrm ->
+      open term k u (tm_var a) = tm_var a.
+  Proof.
+    intros.
+    unfold open.
+    simplify_kbindd.
+    normalize_K.
+  Abort.
+
+  Lemma open_term_rw2 : forall (τ : typ LN) (t : term LN),
+      open term k u (tm_abs τ t) =
+        tm_abs (open typ k u τ) (kbindd term k (open_loc k u ⦿ [ktrm]) t).
+  Proof.
+    test_simplification.
+  Qed.
+
+  Lemma open_term_rw3 : forall (t1 t2 : term LN),
+      open term k u (tm_app t1 t2) =
+        tm_app (open term k u t1) (open term k u t2).
+  Proof.
+    test_simplification.
+  Qed.
+
+  Lemma open_term_rw4 : forall (t : term LN),
+      open term k u (tm_tab t) =
+        tm_tab (kbindd term k (open_loc k u ⦿ [ktyp]) t).
+  Proof.
+    test_simplification.
+  Qed.
+
+  Lemma open_term_rw5 : forall (t: term LN) (τ : typ LN),
+      open term k u (tm_tap t τ) =
+        tm_tap (open term k u t) (open typ k u τ).
+  Proof.
+    test_simplification.
+  Qed.
+
+End rw_open.
+
+Ltac simplify_LCn_pre_refold_hook :=
+  repeat handle_lc_loc.
+
+Ltac simplify_LCn_post_refold_hook :=
+  idtac.
+
+Ltac simplify_LCn :=
+  match goal with
+  | |- context[LCn (T := ?T) (ix := ?ix)
+                ?U ?k ?n ?t] =>
+      rewrite ?(LCn_to_Forallkd _(*U*) (ix := ix));
+      simplify_Forallkd;
+      simplify_LCn_pre_refold_hook;
+      rewrite <- ?(LCn_to_Forallkd _ (ix := ix));
+      simplify_LCn_post_refold_hook
+  end.
+
+(** ** <<LCn>> *)
+(******************************************************************************)
+Section rw_LCn.
+
+  Context
+    (A : Type)
+      (k : K2)
+      (n: nat)
+      (x: atom)
+      (u: SystemF k LN).
+
+  Ltac tactic_being_tested ::= simplify_LCn.
+
+  Lemma LCn_type_rw1 : forall c,
+      LCn typ k n (ty_c c) = True.
+  Proof.
+    test_simplification.
+  Qed.
+
+  (*
+  Lemma LCn_type_rw2_neq : forall (a : A),
+      k <> ktyp ->
+      LC typ k f (ty_v a) = ty_v a.
+  Proof.
+    intros.
+    simplify_LC.
+    rewrite btgd_neq; auto.
+  Qed.*)
+
+  Lemma LCn_type_rw3 : forall (t1 t2 : typ LN),
+      LCn typ k n (ty_ar t1 t2) =
+        (LCn typ k n t1 /\ LCn typ k n t2).
+  Proof.
+    test_simplification.
+  Qed.
+
+  Lemma LCn_type_rw4_eq : forall (body : typ LN),
+      k = ktyp ->
+      LCn typ k n (ty_univ body) =
+        LCn typ k (S n) body.
+  Proof.
+    test_simplification.
+  Qed.
+
+  Lemma LCn_type_rw4_neq : forall (body : typ LN),
+      k <> ktyp ->
+      LCn typ k n (ty_univ body) =
+        LCn typ k n body.
+  Proof.
+    test_simplification.
+  Qed.
+
+  (*
+  Lemma LCn_term_rw1_neq : forall (a : LN),
+      k <> ktrm ->
+      LC term (tm_var a) = tm_var a.
+  Proof.
+    intros.
+    unfold LC.
+    simplify_kbindd.
+    normalize_K.
+  Abort.
+  *)
+
+  Lemma LCn_term_rw2_eq : forall (τ : typ LN) (t : term LN),
+      k = ktrm ->
+      LCn term k n (tm_abs τ t) =
+        (LCn typ k n τ /\ LCn term k (S n) t).
+  Proof.
+    test_simplification.
+  Qed.
+
+  Lemma LCn_term_rw2_neq : forall (τ : typ LN) (t : term LN),
+      k <> ktrm ->
+      LCn term k n (tm_abs τ t) =
+        (LCn typ k n τ /\ LCn term k n t).
+  Proof.
+    test_simplification.
+  Qed.
+
+  Lemma LCn_term_rw3 : forall (t1 t2 : term LN),
+      LCn term k n (tm_app t1 t2) =
+        (LCn term k n t1 /\ LCn term k n t2).
+  Proof.
+    test_simplification.
+  Qed.
+
+  Lemma LCn_term_rw4_neq : forall (t : term LN),
+      k <> ktyp ->
+      LCn term k n (tm_tab t) =
+        LCn term k n t.
+  Proof.
+    test_simplification.
+  Qed.
+
+  Lemma LCn_term_rw4_eq : forall (t : term LN),
+      k = ktyp ->
+      LCn term k n (tm_tab t) =
+        LCn term k (S n) t.
+  Proof.
+    test_simplification.
+  Qed.
+
+  Lemma LCn_term_rw5 : forall (t: term LN) (τ : typ LN),
+      LCn term k n (tm_tap t τ) =
+        (LCn term k n t /\ LCn typ k n τ).
+  Proof.
+    test_simplification.
+  Qed.
+
+End rw_LCn.
+
+Ltac simplify_LC_pre_refold_hook :=
+  idtac.
+
+Ltac simplify_LC_post_refold_hook :=
+  idtac.
+
+Ltac simplify_LC :=
+  match goal with
+  | |- context[LC (T := ?T) (ix := ?ix)
+                ?U ?k ?t] =>
+      unfold LC;
+      simplify_LCn;
+      repeat (change (LCn ?U ?k 0) with (LC U k))
+  end.
+
+(** ** <<LC>> *)
+(******************************************************************************)
+Section rw_LC.
+
+  Context
+    (A : Type)
+      (k : K2)
+      (n: nat)
+      (x: atom)
+      (u: SystemF k LN).
+
+  Ltac tactic_being_tested ::= simplify_LC.
+
+  Lemma LC_type_rw1 : forall c,
+      LC typ k (ty_c c) = True.
+  Proof.
+    test_simplification.
+  Qed.
+
+  Lemma LC_type_rw3 : forall (t1 t2 : typ LN),
+      LC typ k (ty_ar t1 t2) =
+        (LC typ k t1 /\ LC typ k t2).
+  Proof.
+    test_simplification.
+  Qed.
+
+  Lemma LC_type_rw4_eq : forall (body : typ LN),
+      k = ktyp ->
+      LC typ k (ty_univ body) =
+        LCn typ k 1 body.
+  Proof.
+    test_simplification.
+  Qed.
+
+  Lemma LC_type_rw4_neq : forall (body : typ LN),
+      k <> ktyp ->
+      LC typ k (ty_univ body) =
+        LC typ k body.
+  Proof.
+    test_simplification.
+  Qed.
+
+  Lemma LC_term_rw2_eq : forall (τ : typ LN) (t : term LN),
+      k = ktrm ->
+      LC term k (tm_abs τ t) =
+        (LC typ k τ /\ LCn term k 1 t).
+  Proof.
+    test_simplification.
+  Qed.
+
+  Lemma LC_term_rw2_neq : forall (τ : typ LN) (t : term LN),
+      k <> ktrm ->
+      LC term k (tm_abs τ t) =
+        (LC typ k τ /\ LC term k t).
+  Proof.
+    test_simplification.
+  Qed.
+
+  Lemma LC_term_rw3 : forall (t1 t2 : term LN),
+      LC term k (tm_app t1 t2) =
+        (LC term k t1 /\ LC term k t2).
+  Proof.
+    test_simplification.
+  Qed.
+
+  Lemma LC_term_rw4_neq : forall (t : term LN),
+      k <> ktyp ->
+      LC term k (tm_tab t) =
+        LC term k t.
+  Proof.
+    test_simplification.
+  Qed.
+
+  Lemma LC_term_rw4_eq : forall (t : term LN),
+      k = ktyp ->
+      LC term k (tm_tab t) =
+        LCn term k 1 t.
+  Proof.
+    test_simplification.
+  Qed.
+
+  Lemma LC_term_rw5 : forall (t: term LN) (τ : typ LN),
+      LC term k (tm_tap t τ) =
+        (LC term k t /\ LC typ k τ).
+  Proof.
+    test_simplification.
+  Qed.
+
+End rw_LC.
+
+Ltac simplify_subst_pre_refold_hook :=
+  idtac.
+
+Ltac simplify_subst_post_refold_hook :=
+  idtac.
+
+Ltac simplify_subst :=
+  match goal with
+  | |- context[subst (T := ?T) (ix := ?ix)
+                ?U ?k ?t] =>
+      rewrite ?(subst_to_kbind);
+      simplify_kbind;
+      rewrite <- ?(subst_to_kbind)
+  end.
+
+(** ** <<subst>> *)
+(******************************************************************************)
+Section rw_subst.
+
+  Context
+    (A : Type)
+      (k : K2)
+      (n: nat)
+      (x: atom)
+      (u: SystemF k LN).
+
+  Ltac tactic_being_tested ::= simplify_subst.
+
+  Lemma subst_type_rw1 : forall c,
+      subst typ k x u (ty_c c) = ty_c c.
+  Proof.
+    test_simplification.
+  Qed.
+
+  Lemma subst_type_rw3 : forall (t1 t2 : typ LN),
+      subst typ k x u (ty_ar t1 t2) =
+        ty_ar (subst typ k x u t1) (subst typ k x u t2).
+  Proof.
+    test_simplification.
+  Qed.
+
+  Lemma subst_type_rw4 : forall (body : typ LN),
+      subst typ k x u (ty_univ body) =
+        ty_univ (subst typ k x u body).
+  Proof.
+    test_simplification.
+  Qed.
+
+  Lemma subst_term_rw2_eq : forall (τ : typ LN) (t : term LN),
+      subst term k x u (tm_abs τ t) =
+        tm_abs (subst typ k x u τ) (subst term k x u t).
+  Proof.
+    test_simplification.
+  Qed.
+
+  Lemma subst_term_rw2 : forall (τ : typ LN) (t : term LN),
+      subst term k x u (tm_abs τ t) =
+        tm_abs (subst typ k x u τ) (subst term k x u t).
+  Proof.
+    test_simplification.
+  Qed.
+
+  Lemma subst_term_rw3 : forall (t1 t2 : term LN),
+      subst term k x u (tm_app t1 t2) =
+        tm_app (subst term k x u t1) (subst term k x u t2).
+  Proof.
+    test_simplification.
+  Qed.
+
+  Lemma subst_term_rw4 : forall (t : term LN),
+      subst term k x u (tm_tab t) =
+        tm_tab (subst term k x u t).
+  Proof.
+    test_simplification.
+  Qed.
+
+  Lemma subst_term_rw5 : forall (t: term LN) (τ : typ LN),
+      subst term k x u (tm_tap t τ) =
+        tm_tap (subst term k x u t) (subst typ k x u τ).
+  Proof.
+    test_simplification.
+  Qed.
+
+End rw_subst.
+
+Ltac simplify_free_pre_refold_hook :=
+  idtac.
+
+Ltac simplify_free_post_refold_hook :=
+  unfold_ops @Monoid_op_list;
+  unfold_ops @Monoid_unit_list.
+
+Ltac handle_free_at_leaf :=
+  (match goal with
+   | |- context[EqDec_eq_of_EqDec ?Keq ?k1 ?k2] =>
+       destruct (EqDec_eq_of_EqDec Keq k1 k2);
+       try easy
+   end).
+
+Ltac simplify_free :=
+  match goal with
+  | |- context[free (T := ?T) (ix := ?ix)
+                ?U ?k ?t] =>
+      rewrite ?(free_to_foldMapk _ (ix := ix));
+      simplify_foldMapk;
+      simplify_free_pre_refold_hook;
+      rewrite <- ?(free_to_foldMapk _ (ix := ix));
+      simplify_free_post_refold_hook;
+      try solve [handle_free_at_leaf]
+  end.
+
+(** ** <<free>> *)
+(******************************************************************************)
+Section rw_free.
+
+  Context
+    (A : Type)
+      (k : K2)
+      (n: nat)
+      (x: atom)
+      (u: SystemF k LN).
+
+  Ltac tactic_being_tested ::= simplify_free.
+
+  Lemma free_type_rw1 : forall c,
+      free typ k (ty_c c) = nil.
+  Proof.
+    test_simplification.
+  Qed.
+
+  Lemma free_type_rw2_atom_eq : forall (x: atom),
+      k = ktyp ->
+      free typ k (ty_v (Fr x)) = [ x ].
+  Proof.
+    test_simplification.
+  Qed.
+
+  Lemma free_type_rw2_atom : forall (x: atom),
+      k <> ktyp ->
+      free typ k (ty_v (Fr x)) = [ ].
+  Proof.
+    test_simplification.
+  Qed.
+
+  Lemma free_type_rw2_bound : forall n,
+      free typ k (ty_v (Bd n)) = [ ].
+  Proof.
+    test_simplification.
+  Qed.
+
+  Lemma free_type_rw3 : forall (t1 t2 : typ LN),
+      free typ k (ty_ar t1 t2) =
+        free typ k t1 ++ free typ k t2.
+  Proof.
+    test_simplification.
+  Qed.
+
+  Lemma free_type_rw4 : forall (body : typ LN),
+      free typ k (ty_univ body) =
+        free typ k body.
+  Proof.
+    test_simplification.
+  Qed.
+
+  Lemma free_term_rw2_eq : forall (τ : typ LN) (t : term LN),
+      free term k (tm_abs τ t) =
+        free typ k τ ++ free term k t.
+  Proof.
+    test_simplification.
+  Qed.
+
+  Lemma free_term_rw2 : forall (τ : typ LN) (t : term LN),
+      free term k (tm_abs τ t) =
+        free typ k τ ++ free term k t.
+  Proof.
+    test_simplification.
+  Qed.
+
+  Lemma free_term_rw3 : forall (t1 t2 : term LN),
+      free term k (tm_app t1 t2) =
+        free term k t1 ++ free term k t2.
+  Proof.
+    test_simplification.
+  Qed.
+
+  Lemma free_term_rw4 : forall (t : term LN),
+      free term k (tm_tab t) =
+        free term k t.
+  Proof.
+    test_simplification.
+  Qed.
+
+  Lemma free_term_rw5 : forall (t: term LN) (τ : typ LN),
+      free term k (tm_tap t τ) =
+        free term k t ++ free typ k τ.
+  Proof.
+    test_simplification.
+  Qed.
+
+End rw_free.
+
+Ltac assert_identical_with_atoms :=
+    match goal with
+    | |- ?x [=] ?x =>
+        ltac_trace "Both sides identical:";
+        print_goal
+    end.
+
+Ltac test_simplification_with_atoms :=
+  intros;
+  tactic_being_tested;
+  try normalize_K;
+  now assert_identical_with_atoms.
+
+Ltac simplify_FV_pre_refold_hook :=
+  autorewrite with tea_rw_atoms.
+
+Ltac simplify_FV_post_refold_hook :=
+  idtac.
+
+Ltac simplify_FV :=
+  match goal with
+  | |- context[FV (T := ?T) (ix := ?ix)
+                ?U ?k ?t] =>
+      rewrite ?(FV_to_free _ (ix := ix));
+      simplify_free;
+      simplify_FV_pre_refold_hook;
+      rewrite <- ?(FV_to_free _ (ix := ix));
+      simplify_FV_post_refold_hook
+  end.
+
+(** ** <<FV>> *)
+(******************************************************************************)
+Section rw_FV.
+
+  Context
+    (A : Type)
+      (k : K2)
+      (n: nat)
+      (x: atom)
+      (u: SystemF k LN).
+
+  Ltac tactic_being_tested ::= simplify_FV.
+
+  #[local] Open Scope set_scope.
+
+  Lemma FV_type_rw1 : forall c,
+      FV typ k (ty_c c) [=] ∅.
+  Proof.
+    test_simplification_with_atoms.
+  Qed.
+
+  Lemma FV_type_rw2_atom : forall (x: atom),
+      k = ktyp ->
+      FV typ k (ty_v (Fr x)) [=] {{ x }}.
+  Proof.
+    test_simplification_with_atoms.
+  Qed.
+
+  Lemma FV_type_rw3 : forall (t1 t2 : typ LN),
+      FV typ k (ty_ar t1 t2) [=]
+        FV typ k t1 ∪ FV typ k t2.
+  Proof.
+    test_simplification_with_atoms.
+  Qed.
+
+  Lemma FV_type_rw4 : forall (body : typ LN),
+      FV typ k (ty_univ body) [=]
+        FV typ k body.
+  Proof.
+    test_simplification_with_atoms.
+  Qed.
+
+  Lemma FV_term_rw2_eq : forall (τ : typ LN) (t : term LN),
+      FV term k (tm_abs τ t) [=]
+        FV typ k τ ∪ FV term k t.
+  Proof.
+    test_simplification_with_atoms.
+  Qed.
+
+  Lemma FV_term_rw2 : forall (τ : typ LN) (t : term LN),
+      FV term k (tm_abs τ t) [=]
+        FV typ k τ ∪ FV term k t.
+  Proof.
+    test_simplification_with_atoms.
+  Qed.
+
+  Lemma FV_term_rw3 : forall (t1 t2 : term LN),
+      FV term k (tm_app t1 t2) [=]
+        FV term k t1 ∪ FV term k t2.
+  Proof.
+    test_simplification_with_atoms.
+  Qed.
+
+  Lemma FV_term_rw4 : forall (t : term LN),
+      FV term k (tm_tab t) [=]
+        FV term k t.
+  Proof.
+    test_simplification_with_atoms.
+  Qed.
+
+  Lemma FV_term_rw5 : forall (t: term LN) (τ : typ LN),
+      FV term k (tm_tap t τ) [=]
+        FV term k t ∪ FV typ k τ.
+  Proof.
+    test_simplification_with_atoms.
+  Qed.
+
+End rw_FV.
+
+Ltac simplify_scoped_pre_refold_hook :=
+  idtac.
+
+Ltac simplify_scoped_post_refold_hook :=
+  idtac.
+
+Ltac simplify_scoped :=
+  match goal with
+  | |- context[scoped (T := ?T) (ix := ?ix)
+                ?U ?k ?n ?t] =>
+      idtac
+  end.
+(*
+      rewrite ?(scoped_to_Forallkd _(*U*) (ix := ix));
+      simplify_Forallkd;
+      simplify_scoped_pre_refold_hook;
+      rewrite <- ?(scoped_to_Forallkd _ (ix := ix));
+      simplify_scoped_post_refold_hook
+*)
+
+(** ** <<scoped>> *)
+(******************************************************************************)
+Section rw_scoped.
+
+  Context
+    (A : Type)
+      (k : K2)
+      (Γ : AtomSet.t)
+      (u: SystemF k LN).
+
+  Ltac tactic_being_tested ::= simplify_scoped.
+
+  Lemma scoped_type_rw1 : forall c,
+      scoped typ k (ty_c c) Γ <-> True.
+  Proof.
+    intros.
+    unfold scoped.
+    simplify_FV.
+    split; fsetdec.
+  Qed.
+
+  (*
+  Lemma scoped_type_rw2_neq : forall (a : A),
+      k <> ktyp ->
+      LC typ k f (ty_v a) = ty_v a.
+  Proof.
+    intros.
+    simplify_LC.
+    rewrite btgd_neq; auto.
+  Qed.*)
+
+  Lemma scoped_type_rw3 : forall (t1 t2 : typ LN),
+      scoped typ k (ty_ar t1 t2) Γ <->
+        (scoped typ k t1 Γ /\ scoped typ k t2 Γ).
+  Proof.
+    intros.
+    unfold scoped.
+    simplify_FV.
+    intuition fsetdec.
+  Qed.
+
+  Lemma scoped_type_rw4_eq : forall (body : typ LN),
+      scoped typ k (ty_univ body) Γ <->
+        scoped typ k body Γ.
+  Proof.
+    intros.
+    unfold scoped.
+    simplify_FV.
+    intuition fsetdec.
+  Qed.
+
+  Lemma scoped_type_rw4_neq : forall (body : typ LN),
+      scoped typ k (ty_univ body) =
+        scoped typ k body.
+  Proof.
+    intros.
+    unfold scoped.
+    simplify_FV.
+    conclude.
+  Qed.
+
+  #[local] Open Scope set_scope.
+
+  Lemma scoped_term_rw1_eq : forall (x : atom),
+      k = ktrm ->
+      scoped term k (tm_var (Fr x)) Γ = ({{x}} ⊆ Γ).
+  Proof.
+    intros.
+    unfold scoped.
+    simplify_FV.
+  Qed.
+
+  Lemma scoped_term_rw1_neq : forall (x : atom),
+      k <> ktrm ->
+      scoped term k (tm_var (Fr x)) Γ = True.
+  Proof.
+    intros.
+    unfold scoped.
+    propext; simplify_FV.
+  Qed.
+
+  Lemma scoped_term_rw2: forall (τ : typ LN) (t : term LN),
+      scoped term k (tm_abs τ t) Γ <->
+        (scoped typ k τ Γ /\ scoped term k t Γ).
+  Proof.
+    intros.
+    unfold scoped.
+    simplify_FV.
+    intuition fsetdec.
+  Qed.
+
+  Lemma scoped_term_rw3 : forall (t1 t2 : term LN),
+      scoped term k (tm_app t1 t2) Γ <->
+        (scoped term k t1 Γ /\ scoped term k t2 Γ).
+  Proof.
+    intros.
+    unfold scoped.
+    simplify_FV.
+    intuition fsetdec.
+  Qed.
+
+  Lemma scoped_term_rw4_neq : forall (t : term LN),
+      scoped term k (tm_tab t) Γ <->
+        scoped term k t Γ.
+  Proof.
+    intros.
+    unfold scoped.
+    simplify_FV.
+    intuition fsetdec.
+  Qed.
+
+  Lemma scoped_term_rw4_eq : forall (t : term LN),
+      scoped term k (tm_tab t) Γ <->
+        scoped term k t Γ.
+  Proof.
+    intros.
+    unfold scoped.
+    simplify_FV.
+    intuition fsetdec.
+  Qed.
+
+  Lemma scoped_term_rw5 : forall (t: term LN) (τ : typ LN),
+      scoped term k (tm_tap t τ) Γ <->
+        (scoped term k t Γ /\ scoped typ k τ Γ).
+  Proof.
+    intros.
+    unfold scoped.
+    simplify_FV.
+    intuition fsetdec.
+  Qed.
+
+End rw_scoped.
